ss[12pt]{article}
\usepackage[utf8]{amsmath}
\usepackage[utf8]{amssymb}

\title{Euler's Formula\&Equation Proofs Using Taylor Series}

\begin{document}
\maketitle

\begin{equation}
e^{x} &= 1 + x + \frac{x^{2}}{2!} + \frac{x^{3}}{3!} + ...
\end{equation}

\begin{equation}
\sin(x) &= x - \frac{x^{3}}{3!} + \frac{x^{5}}{5!} - \frac{x^{7}}{7!} + ...
\end{equation}

\begin{equation}
\cos(x) &= 1 - \frac{x^{2}}{2!} + \frac{x^{4}}{4!} - \frac{x^{6}}{6!} + ...
\end{equation}

\begin{proof}
So,
	\begin{align}
	e^{ix} &= 1 + ix - \frac{x^2}{2!} - \frac{ix^3}{3!} +
	\frac{x^4}{4!} +
	\frac{ix^5}{5!} - 
	\frac{x^6}{6!} -
	\frac{ix^7}{7!} + ... \\
		&= (1 - \frac{x^2}{2!} + \frac{x^4}{4!} - \frac{x^6}{6!} + \frac{x^8}{8!} - ...) +
		i(x - \frac{x^3}{3!} + \frac{x^5}{5!} - \frac{x^7}{7!} + ...) \\
			&= \cos(x) + i\sin(x).
	\end{align}
\end{proof}
This is Euler's formular

now, In Euler's formula, let's put $\pi$ in $x$
\begin{equation}
	\cos(\pi) &= -1 
\end{equation}

\begin{equation}
	\sin(\pi) &= 0, 
\end{equation}

\begin{equation}
	e^{i\pi} &= -1 + 0i 
\end{equation}

\begin{equation}
	e^{i\pi} + 1 &= 0 
\end{equation}

\end{document}


